\documentclass{article}

% Language setting
% Replace `english' with e.g. `spanish' to change the document language
\usepackage[english]{babel}

% Set page size and margins
% Replace `letterpaper' with `a4paper' for UK/EU standard size
\usepackage[letterpaper,top=2cm,bottom=2cm,left=3cm,right=3cm,marginparwidth=1.75cm]{geometry}

% Useful packages
\usepackage{amsmath}
\usepackage{graphicx}
\usepackage[colorlinks=true, allcolors=blue]{hyperref}
\usepackage{amssymb}

\title{Algebra}
\date{}

\begin{document}
\maketitle

\tableofcontents

\newpage
\section{Quadratic Equation}

\[
    ax^2 + bx + c = 0
\]
\[
    x = \frac{-b \pm \sqrt{b^2 - 4ac}}{2a}
\]

\subsection{Vieta's Formulas}
\[
    x_1 + x_2 = -\frac{b}{a}
\]
\[
    x_1 x_2 = \frac{c}{a}
\]


\newpage
\section{Polynomial Identities}

\subsection{Cube Formulas}
\[
    (a + b)^3 = a^3 + 3a^2b + 3ab^2 + b^3
\]
\[
    a^3 + b^3 = (a + b)(a^2 - ab + b^2)
\]
\[
    a^3 - b^3 = (a - b)(a^2 + ab + b^2)
\]


\newpage
\section{Inequalities}

\subsection{HM-GM-AM-QM Inequalities}
\[
    f(x) = \left(\frac{a^x + b^x}{2}\right)^{\frac{1}{x}}
\]
\[
    \frac{2}{\frac{1}{a} + \frac{1}{b}} \le \sqrt{ab} \le \frac{a + b}{2} \le \sqrt{\frac{a^2 + b^2}{2}}
\]


\newpage
\section{Exponential Function}

\[
    a^m \cdot a^n = a^{m+n}
\]
\[
    \frac{a^m}{a^n} = a^{m-n}
\]
\[
    (a^m)^n = a^{m \cdot n}
\]
\[
    (ab)^n = a^n \cdot b^n
\]
\[
    \left(\frac{a}{b}\right)^n = \frac{a^n}{b^n}
\]
\[
    a^0 = 1 \quad (a \neq 0)
\]
\[
    a^{-n} = \frac{1}{a^n}
\]
\[
    a^{\frac{m}{n}} = \sqrt[n]{a^m}
\]


\newpage
\section{Logarithm Function}

\[
    \log(MN) = \log M + \log N
\]
\[
    \log\frac{M}{N} = \log M - \log N
\]
\[
    \log M^p = p \log M
\]
\[
    \log_b M = \frac{\log_k M}{\log_k b}
\]
\[
    b^{\log_b M} = M
\]
\[
    \log_b b^x = x
\]


\newpage
\section{Sequence}

\subsection{Arithmetic Sequence}

\subsubsection{General Term Formula}
\[
    a_n = a_1 + (n-1)d
\]
\[
    a_n = a_m + (n-m)d
\]

\subsubsection{Sum of Terms}
\[
    S_n = \frac{n(a_1 + a_n)}{2}
\]
\[
    S_n = na_1 + \frac{n(n-1)d}{2}
\]

\subsubsection{Properties}
\[
    m + n = p + q \Rightarrow a_m + a_n = a_p + a_q
\]

\subsection{Geometric Sequence}

\subsubsection{General Term Formula}
\[
    a_n = a_1 \cdot r^{n-1}
\]
\[
    a_n = a_m \cdot r^{n-m}
\]

\subsubsection{Sum of Terms}
When $r = 1$:
\[
    S_n = n \cdot a_1
\]
When $r \neq 1$:
\[
    S_n = \frac{a_1(1 - r^n)}{1 - r}
\]

\subsubsection{Properties}
\[
    m + n = p + q \Rightarrow a_m \cdot a_n = a_p \cdot a_q
\]

\end{document}
