\documentclass{article}

% Language setting
% Replace `english' with e.g. `spanish' to change the document language
\usepackage[english]{babel}

% Set page size and margins
% Replace `letterpaper' with `a4paper' for UK/EU standard size
\usepackage[letterpaper,top=2cm,bottom=2cm,left=3cm,right=3cm,marginparwidth=1.75cm]{geometry}

% Useful packages
\usepackage{amsmath}
\usepackage{graphicx}
\usepackage[colorlinks=true, allcolors=blue]{hyperref}
\usepackage{amssymb}

\title{Calculus}
\date{}

\begin{document}
\maketitle

\tableofcontents

\newpage
\section{Single Variable Calculus}

\subsection{Limit}

\[
    \lim_{x \to 0} \frac{\sin x}{x} = 1
\]
\[
    \lim_{x \to \infty} \left(1 + \frac{1}{x}\right)^x = e
\]
\[
    \lim_{x \to \infty} \left(1 + \frac{\lambda}{x}\right)^x = e^\lambda
\]

\subsection{Equivalent Infinitesimal}

\[
    \sin x \sim x
\]
\[
    1 - \cos x \sim \frac{x^2}{2}
\]
\[
    \arcsin x \sim x
\]
\[
    \tan x \sim x
\]
\[
    \arctan x \sim x
\]
\[
    e^x - 1 \sim x
\]
\[
    a^x - 1 \sim x \ln a
\]
\[
    \ln(1 + x) \sim x
\]
\[
    \log_a(1 + x) \sim \frac{x}{\ln a}
\]
\[
    (1 + ax)^b - 1 \sim abx
\]

\subsection{Derivative}

\subsubsection{Basic Functions}

\[
    \frac{d}{dx} x^a = ax^{a-1}
\]
\[
    \frac{d}{dx} e^x = e^x
\]
\[
    \frac{d}{dx} a^x = a^x \ln a
\]
\[
    \frac{d}{dx} \ln x = \frac{1}{x}
\]
\[
    \frac{d}{dx} \log_a x = \frac{1}{x \ln a}
\]
\[
    \frac{d}{dx} \sin x = \cos x
\]
\[
    \frac{d}{dx} \cos x = -\sin x
\]
\[
    \frac{d}{dx} \tan x = \sec^2 x
\]
\[
    \frac{d}{dx} \cot x = -\csc^2 x
\]
\[
    \frac{d}{dx} \sec x = \sec x \tan x
\]
\[
    \frac{d}{dx} \csc x = -\csc x \cot x
\]
\[
    \frac{d}{dx} \arcsin x = \frac{1}{\sqrt{1 - x^2}}
\]
\[
    \frac{d}{dx} \arccos x = -\frac{1}{\sqrt{1 - x^2}}
\]
\[
    \frac{d}{dx} \arctan x = \frac{1}{1 + x^2}
\]
\[
    \frac{d}{dx} \operatorname{arccot} x = -\frac{1}{1 + x^2}
\]

\subsubsection{Combined Functions}

\[
    (\alpha f + \beta g)' = \alpha f' + \beta g'
\]
\[
    (fg)' = f'g + fg'
\]
\[
    \left(\frac{f}{g}\right)' = \frac{f'g - fg'}{g^2}
\]

\subsubsection{Chain Rule}

\[
    f'(g(x)) = f'(g(x)) \cdot g'(x)
\]

\subsubsection{Inverse Function}

\[
    (f^{-1})'(x) = \frac{1}{f'(f^{-1}(x))}
\]

\subsubsection{Parametric Functions}

\[
    \begin{cases}
        y = y(t) \\
        x = x(t)
    \end{cases}
\]
\[
    \frac{dy}{dx} = \frac{\frac{dy}{dt}}{\frac{dx}{dt}}
\]
\[
    \frac{d^2y}{dx^2} = \frac{d\frac{dy}{dx}}{dt} \cdot \frac{dt}{dx}
\]

\subsubsection{Implicit Function}

\[
    F(x, y) = 0
\]
\[
    \frac{dy}{dx} = -\frac{F_x'}{F_y'}
\]

\subsubsection{Definite Integral with Variable Bounds}

\[
    \frac{d}{dx} \int_a^x f(t) dt = f(x)
\]

\subsection{L'HÃ´pital's Rule}

If $\lim_{x \to c} f(x) = \lim_{x \to c} g(x) = 0$ or $\pm\infty$:
\[
    \lim_{x \to c} \frac{f(x)}{g(x)} = \lim_{x \to c} \frac{f'(x)}{g'(x)}
\]

\subsection{Taylor Series}

\[
    f(x) = \sum_{n=0}^{\infty} \frac{f^{(n)}(a)}{n!}(x - a)^n
\]
Let $h = x - a$:
\[
    f(a + h) = \sum_{n=0}^{\infty} \frac{f^{(n)}(a)}{n!}h^n
\]

\subsubsection{Exponential Function}

\[
    e^x = \sum_{n=0}^{\infty} \frac{x^n}{n!}
\]

\subsubsection{Natural Logarithm}

\[
    \ln(1 - x) = -\sum_{n=1}^{\infty} \frac{x^n}{n}
\]
\[
    \ln(1 + x) = \sum_{n=1}^{\infty} (-1)^{n+1} \frac{x^n}{n}
\]

\subsubsection{Binomial Series}

\[
    (1 + x)^\alpha = \sum_{n=0}^{\infty} \binom{\alpha}{n} x^n
\]

\subsubsection{Trigonometric Functions}

\[
    \sin x = \sum_{n=0}^{\infty} \frac{(-1)^n}{(2n + 1)!} x^{2n + 1}
\]
\[
    \cos x = \sum_{n=0}^{\infty} \frac{(-1)^n}{(2n)!} x^{2n}
\]

\subsection{Applications for Derivatives}

\subsubsection{Tangent Line Equation}

\[
    y - y_0 = y'(x - x_0)
\]

\subsubsection{Extrema}

\[
    y' = 0
\]

\subsubsection{Arc Length}

\[
    ds = \sqrt{1 + (y')^2} dx
\]

\subsubsection{Curvature}

\[
    \kappa = \frac{|y''|}{(1 + (y')^2)^{3/2}}
\]
For parametric equations:
\[
    \kappa = \frac{|\phi'(t)\psi''(t) - \phi''(t)\psi'(t)|}{(\phi'(t)^2 + \psi'(t)^2)^{3/2}}
\]

\subsubsection{Radius of Curvature}

\[
    \rho = \frac{1}{\kappa}
\]

\subsubsection{Center of Curvature}

\[
    D(\alpha, \beta)
\]
\[
    \begin{cases}
        \alpha = x - \frac{y'(1 + (y')^2)}{y''} \\
        \beta = y + \frac{1 + (y')^2}{y''}
    \end{cases}
\]

\subsection{Integrals}

\subsubsection{Indefinite Integrals}

\textbf{Rational Functions:}
\[
    \int a dx = ax + C
\]
\[
    \int x^n dx = \frac{x^{n+1}}{n+1} + C \quad (n \neq -1)
\]
\[
    \int (ax + b)^n dx = \frac{(ax + b)^{n+1}}{a(n+1)} + C \quad (n \neq -1)
\]
\[
    \int \frac{1}{x} dx = \ln|x| + C
\]
\[
    \int \frac{c}{ax + b} dx = \frac{c}{a} \ln|ax + b| + C
\]
\textbf{Exponential Functions:}
\[
    \int e^{ax} dx = \frac{1}{a} e^{ax} + C
\]
\[
    \int f'(x) e^{f(x)} dx = e^{f(x)} + C
\]
\[
    \int a^x dx = \frac{a^x}{\ln a} + C
\]
\textbf{Logarithms:}
\[
    \int \ln x dx = x \ln x - x + C
\]
\[
    \int \log_a x dx = x \log_a x - \frac{x}{\ln a} + C = \frac{x \ln x - x}{\ln a} + C
\]
\textbf{Trigonometric Functions:}
\[
    \int \sin x dx = -\cos x + C
\]
\[
    \int \cos x dx = \sin x + C
\]
\[
    \int \tan x dx = -\ln|\cos x| + C
\]
\[
    \int \cot x dx = \ln|\sin x| + C
\]
\[
    \int \sec x dx = \ln|\sec x + \tan x| + C
\]
\[
    \int \csc x dx = -\ln|\csc x + \cot x| + C
\]
\[
    \int \sec^2 x dx = \tan x + C
\]
\[
    \int \csc^2 x dx = -\cot x + C
\]
\[
    \int \sec x \tan x dx = \sec x + C
\]
\[
    \int \csc x \cot x dx = -\csc x + C
\]
\[
    \int \sin^2 x dx = \frac{1}{2}\left(x - \frac{\sin 2x}{2}\right) + C
\]
\[
    \int \cos^2 x dx = \frac{1}{2}\left(x + \frac{\sin 2x}{2}\right) + C
\]
\[
    \int \tan^2 x dx = \tan x - x + C
\]
\[
    \int \cot^2 x dx = -\cot x - x + C
\]
\[
    \int \sec^3 x dx = \frac{1}{2}\left(\sec x \tan x + \ln|\sec x + \tan x|\right) + C
\]
\[
    \int \csc^3 x dx = \frac{1}{2}\left(-\csc x \cot x + \ln|\csc x - \cot x|\right) + C
\]
\[
    \int \sin^n x dx = -\frac{\sin^{n-1} x \cos x}{n} + \frac{n-1}{n} \int \sin^{n-2} x dx
\]
\[
    \int \cos^n x dx = \frac{\cos^{n-1} x \sin x}{n} + \frac{n-1}{n} \int \cos^{n-2} x dx
\]
\textbf{Inverse Trigonometric Functions:}
\[
    \int \arcsin x dx = x \arcsin x + \sqrt{1 - x^2} + C
\]
\[
    \int \arccos x dx = x \arccos x - \sqrt{1 - x^2} + C
\]
\[
    \int \arctan x dx = x \arctan x - \frac{1}{2} \ln|1 + x^2| + C
\]
\[
    \int \operatorname{arccot} x dx = x \operatorname{arccot} x + \frac{1}{2} \ln|1 + x^2| + C
\]
\[
    \int \operatorname{arcsec} x dx = x \operatorname{arcsec} x - \ln|x(1 + \sqrt{1 - x^{-2}})| + C
\]
\[
    \int \operatorname{arccsc} x dx = x \operatorname{arccsc} x + \ln|x(1 + \sqrt{1 - x^{-2}})| + C
\]

\subsubsection{Definite Integrals}

\[
    \int_0^{\pi/2} \sin^n x dx = \int_0^{\pi/2} \cos^n x dx = \frac{(n-1)!!}{n!!} \times
    \begin{cases}
        1 & \text{if } n \text{ is odd} \\
        \frac{\pi}{2} & \text{if } n \text{ is even}
    \end{cases}
\]

\subsection{Ordinary Differential Equations}

\subsubsection{Separable Differential Equation}

\[
    P(x) dx = Q(y) dy
\]
\[
    \int P(x) dx = \int Q(y) dy
\]

\subsubsection{Homogeneous Differential Equation}

\[
    \frac{dy}{dx} = F\left(\frac{y}{x}\right)
\]
Set $u = \frac{y}{x}$, $\frac{dy}{dx} = u + x\frac{du}{dx}$:
\[
    u + x\frac{du}{dx} = F(u)
\]
\[
    \frac{1}{F(u) - u} du = \frac{1}{x} dx
\]

\subsubsection{First Order Linear Differential Equation}

\[
    y' + P(x)y = Q(x)
\]
\[
    y = e^{-\int P(x) dx} \left(\int Q(x) e^{\int P(x) dx} dx + C\right)
\]

\subsubsection{Bernoulli Equation}

\[
    y' + P(x)y = Q(x)y^n \quad (n \neq 0, 1)
\]
\[
    y^{-n} \frac{dy}{dx} + P(x) y^{1-n} = Q(x)
\]
Set $z = y^{1-n}$:
\[
    \frac{dz}{dx} = (1-n) y^{-n} \frac{dy}{dx}
\]

\[
    \frac{dz}{dx} + (1-n)P(x)z = (1-n)Q(x)
\]

\subsubsection{Higher Order Linear Differential Equations}

\textbf{Degradable Higher Order Differential Equations:}

\begin{itemize}
    \item $y^{(n)} = f(x)$
    \[
        y = \underbrace{\int \int \cdots \int}_{n \text{ times}} f(x) dx
    \]

    \item $y'' = f(x, y')$

    Set $y' = p$:
    \[
        y'' = \frac{dp}{dx} = p'
    \]
    \[
        p' = f(x, p)
    \]

    \item $y'' = f(y, y')$

    Set $y' = p$:
    \[
        y'' = \frac{dp}{dx} = \frac{dp}{dy} \frac{dy}{dx} = p \frac{dp}{dy}
    \]
    \[
        p \frac{dp}{dy} = f(y, p)
    \]
\end{itemize}

\textbf{Homogeneous Linear Differential Equations with Constant Coefficients:}

\[
    y'' + py' + qy = 0
\]

Characteristic Equation: $r^2 + pr + q = 0$

\begin{itemize}
    \item $r_1 \neq r_2$: $y = C_1 e^{r_1 x} + C_2 e^{r_2 x}$
    \item $r_1 = r_2$: $y = (C_1 + C_2 x) e^{r_1 x}$
    \item $r_{1,2} = \alpha \pm \beta i$: $y = e^{\alpha x}(C_1 \cos \beta x + C_2 \sin \beta x)$
\end{itemize}

\textbf{Inhomogeneous Linear Differential Equations with Constant Coefficients:}

\[
    y'' + py' + qy = f(x)
\]
\[
    y = Y(x) + y^*(x)
\]

\begin{itemize}
    \item $f(x) = e^{\lambda x} P_m(x)$
    \[
        y^* = x^k R_m(x) e^{\lambda x}
    \]

    where $k$ is the multiplicity of $\lambda$ as a root of the characteristic equation.

    \item $f(x) = e^{\lambda x}(P_l(x) \cos \omega x + Q_n(x) \sin \omega x)$
    \[
        y^* = x^k e^{\lambda x}(R_m^{(1)}(x) \cos \omega x + R_m^{(2)}(x) \sin \omega x)
    \]

    where $m = \max\{l, n\}$ and $k$ is the multiplicity of $\lambda + \omega i$ as a root of the characteristic equation.
\end{itemize}

\newpage
\section{Multivariable Calculus}

\subsection{Total Differential}

\[
    df = \sum_{i=1}^n \frac{\partial f}{\partial x_i} dx_i
\]

\subsection{Numerator Layout}

$f: \mathbb{R}^n \to \mathbb{R}^m$, $Y = f(X)$
\[
    \left[\frac{\partial Y}{\partial X}\right]_{i,j} = \frac{\partial Y_{i}}{\partial X_{j}}
\]
\[
    \frac{\partial Y}{\partial X} \in \mathbb{R}^{m\times n}
\]


\subsection{Derivative of Scalar-valued Function}

$f: \mathbb{R}^n \to \mathbb{R}$, $f = f(\mathbf{x})$

\subsubsection{Gradient}

\[
    \nabla f = \frac{\partial f}{\partial \mathbf{x}^T} =
    \begin{bmatrix}
        \frac{\partial f}{\partial x_1} \\
        \vdots \\
        \frac{\partial f}{\partial x_n}
    \end{bmatrix}
\]

\subsubsection{Hessian Matrix}
Curvature of a function.
\[
    \mathbf{H} = \nabla^2 f =
    \begin{bmatrix}
        \frac{\partial^2 f}{\partial x_1^2} & \cdots & \frac{\partial^2 f}{\partial x_1 \partial x_n} \\
        \vdots & \ddots & \vdots \\
        \frac{\partial^2 f}{\partial x_n \partial x_1} & \cdots & \frac{\partial^2 f}{\partial x_n^2}
    \end{bmatrix}
\]
The Jacobian matrix of the Gradient of $f$.
\[
    \mathbf{H}(f) = \mathbf{J}(\nabla f)
\]

\subsubsection{Chain Rule}

\subsection{Derivative of Vector-valued Function}

$\mathbf{f}: \mathbb{R}^n \to \mathbb{R}^m$, $\mathbf{f}(\mathbf{x}) = \mathbf{y}$

\subsubsection{Jacobian Matrix}

\[
    \mathbf{J} = \frac{\partial \mathbf{f}}{\partial \mathbf{x}} =
    \begin{bmatrix}
        \frac{\partial y_1}{\partial x_1} & \cdots & \frac{\partial y_1}{\partial x_n} \\
        \vdots & \ddots & \vdots \\
        \frac{\partial y_m}{\partial x_1} & \cdots & \frac{\partial y_m}{\partial x_n}
    \end{bmatrix}
\]

\subsection{Chain Rule}

$f = f(\mathbf{x}(\mathbf{t}))$
\[
    \frac{\partial f}{\partial t_j} = \sum_{i=1}^n \frac{\partial f}{\partial x_i} \frac{\partial x_i}{\partial t_j}
\]
\[
    \nabla_{\mathbf{t}} f = \mathbf{J}_{\mathbf{x} \to \mathbf{t}}^T \cdot \nabla_{\mathbf{x}} f
\]
$\mathbf{y} = \mathbf{f}(\mathbf{x}(\mathbf{t}))$
\[
    \frac{\partial \mathbf{y}}{\partial t_j} = \sum_{i=1}^n \frac{\partial \mathbf{y}}{\partial x_i} \frac{\partial x_i}{\partial t_j}
\]
\[
    \mathbf{J}_{\mathbf{y} \to \mathbf{t}} = \mathbf{J}_{\mathbf{y} \to \mathbf{x}} \cdot \mathbf{J}_{\mathbf{x} \to \mathbf{t}}
\]

\subsection{Directional Derivative}

\[
    \nabla_u f(x) = \hat{u} \cdot \nabla f(x)
\]

\subsection{Implicit Function}

\[
    F(x, y, z) = 0
\]
\[
    \frac{\partial z}{\partial x} = -\frac{F_x'}{F_z'}
\]
\[
    \frac{\partial z}{\partial y} = -\frac{F_y'}{F_z'}
\]

\subsection{Jacobian Determinant}

\[
    \det(\mathbf{J}) = \left|\frac{\partial y}{\partial x}\right| = \begin{vmatrix}
        \frac{\partial y_1}{\partial x_1} & \cdots & \frac{\partial y_1}{\partial x_n} \\
        \vdots & \ddots & \vdots \\
        \frac{\partial y_m}{\partial x_1} & \cdots & \frac{\partial y_m}{\partial x_n}
    \end{vmatrix}
\]
\[
    dx = \left|\frac{\partial x}{\partial u}\right| du
\]

\subsection{System of Functions}

\[
    \begin{cases}
        F(x, y, u(x, y), v(x, y)) = 0 \\
        G(x, y, u(x, y), v(x, y)) = 0
    \end{cases}
\]
\[
    \det(\mathbf{J}) = \frac{\partial(F, G)}{\partial(u, v)}
\]
\[
    \frac{\partial u}{\partial x} = -\frac{1}{\det(\mathbf{J})} \frac{\partial(F, G)}{\partial(x, v)} = -\frac{\begin{vmatrix} F_x' & F_v' \\ G_x' & G_v' \end{vmatrix}}{\begin{vmatrix} F_u' & F_v' \\ G_u' & G_v' \end{vmatrix}}
\]
\[
    \frac{\partial v}{\partial x} = -\frac{1}{\det(\mathbf{J})} \frac{\partial(F, G)}{\partial(u, x)} = -\frac{\begin{vmatrix} F_u' & F_x' \\ G_u' & G_x' \end{vmatrix}}{\begin{vmatrix} F_u' & F_v' \\ G_u' & G_v' \end{vmatrix}}
\]
\[
    \frac{\partial u}{\partial y} = -\frac{1}{\det(\mathbf{J})} \frac{\partial(F, G)}{\partial(y, v)} = -\frac{\begin{vmatrix} F_y' & F_v' \\ G_y' & G_v' \end{vmatrix}}{\begin{vmatrix} F_u' & F_v' \\ G_u' & G_v' \end{vmatrix}}
\]
\[
    \frac{\partial v}{\partial y} = -\frac{1}{\det(\mathbf{J})} \frac{\partial(F, G)}{\partial(u, y)} = -\frac{\begin{vmatrix} F_u' & F_y' \\ G_u' & G_y' \end{vmatrix}}{\begin{vmatrix} F_u' & F_v' \\ G_u' & G_v' \end{vmatrix}}
\]

\subsection{Hessian Determinant}

For $f(x, y)$:

\[
    \det(\mathbf{H}) = \begin{vmatrix}
        \frac{\partial^2 f}{\partial x_1^2} & \frac{\partial^2 f}{\partial x_1 x_2} \\
        \frac{\partial^2 f}{\partial x_2 x_1} & \frac{\partial^2 f}{\partial x_2^2}
    \end{vmatrix}
\]

\subsection{Taylor Series}

\[
    f(\mathbf{x}) = \sum_{|\boldsymbol{\alpha}|=0}^{\infty} \frac{D^{\boldsymbol{\alpha}} f(\mathbf{a})}{\boldsymbol{\alpha}!} (\mathbf{x} - \mathbf{a})^{\boldsymbol{\alpha}}
\]
where:
\begin{itemize}
    \item $\mathbf{x} = (x_1, x_2, \ldots, x_n) \in \mathbb{R}^n$ is the variable vector
    \item $\mathbf{a} = (a_1, a_2, \ldots, a_n) \in \mathbb{R}^n$ is the expansion point
    \item $\boldsymbol{\alpha} = (\alpha_1, \alpha_2, \ldots, \alpha_n)$ is a multi-index with $\alpha_i \geq 0$ for all $i$
    \item $|\boldsymbol{\alpha}| = \alpha_1 + \alpha_2 + \cdots + \alpha_n$ is the order of the multi-index
    \item $\boldsymbol{\alpha}! = \alpha_1! \alpha_2! \cdots \alpha_n!$ is the multi-index factorial
    \item $(\mathbf{x} - \mathbf{a})^{\boldsymbol{\alpha}} = (x_1 - a_1)^{\alpha_1} (x_2 - a_2)^{\alpha_2} \cdots (x_n - a_n)^{\alpha_n}$
    \item $D^{\boldsymbol{\alpha}} f(\mathbf{a}) = \frac{\partial^{|\boldsymbol{\alpha}|} f}{\partial x_1^{\alpha_1} \partial x_2^{\alpha_2} \cdots \partial x_n^{\alpha_n}}\bigg|_{\mathbf{x}=\mathbf{a}}$ is the mixed partial derivative of order $|\boldsymbol{\alpha}|$ evaluated at $\mathbf{a}$
\end{itemize}
Let $\mathbf{h} = \mathbf{x} - \mathbf{a}$:
\[
    f(\mathbf{a} + \mathbf{h}) = \sum_{|\boldsymbol{\alpha}|=0}^{\infty} \frac{D^{\boldsymbol{\alpha}} f(\mathbf{a})}{\boldsymbol{\alpha}!} \mathbf{h}^{\boldsymbol{\alpha}}
\]

\subsubsection{Second Order Taylor Series}
\[
    f(\mathbf{x}) \approx f(\mathbf{a}) + \nabla f(\mathbf{a})^T (\mathbf{x}-\mathbf{a}) + \frac{1}{2} (\mathbf{x}-\mathbf{a})^T \mathbf{H}(\mathbf{a}) (\mathbf{x}-\mathbf{a})
\]
Let $\mathbf{h} = \mathbf{x} - \mathbf{a}$:
\[
    f(\mathbf{a} + \mathbf{h}) \approx f(\mathbf{a}) + \nabla f(\mathbf{a})^T \mathbf{h} + \frac{1}{2} \mathbf{h}^T \mathbf{H}(\mathbf{a}) \mathbf{h}
\]

\subsection{Applications for Bivariable Derivatives}

\subsubsection{Tangent Line Equation}

\begin{itemize}
    \item For parametric curve:
    \[
        \begin{cases}
            x = \phi(t) \\
            y = \psi(t) \\
            z = \omega(t)
        \end{cases}
    \]
    \[
        \frac{x - x_0}{\phi'(t_0)} = \frac{y - y_0}{\psi'(t_0)} = \frac{z - z_0}{\omega'(t_0)}
    \]

    \item For intersection of surfaces:
    \[
        \begin{cases}
            F(x, y, z) = 0 \\
            G(x, y, z) = 0
        \end{cases}
    \]
    \[
        \frac{x - x_0}{\begin{vmatrix} F_y' & F_z' \\ G_y' & G_z' \end{vmatrix}_M} = \frac{y - y_0}{\begin{vmatrix} F_z' & F_x' \\ G_z' & G_x' \end{vmatrix}_M} = \frac{z - z_0}{\begin{vmatrix} F_x' & F_y' \\ G_x' & G_y' \end{vmatrix}_M}
    \]
\end{itemize}

\subsubsection{Normal Plane Equation}

For $F(x, y, z) = 0$:
\[
    F_x'(x_0, y_0, z_0)(x - x_0) + F_y'(x_0, y_0, z_0)(y - y_0) + F_z'(x_0, y_0, z_0)(z - z_0) = 0
\]

\subsubsection{Critical Points}

\[
    \nabla f = \mathbf{0}
\]

\begin{itemize}
    \item \textbf{Local Minimum}: $\mathbf{H} \succ 0$ (all eigenvalues $> 0$)
    \item \textbf{Local Maximum}: $\mathbf{H} \prec 0$ (all eigenvalues $< 0$)
    \item \textbf{Saddle Point}: $\mathbf{H}$ has both positive and negative eigenvalues
    \item \textbf{Degenerate}: $\mathbf{H}$ has zero eigenvalues
\end{itemize}

\subsubsection{Conditional Extrema}

\[
    L(x, y) = f(x, y) + \lambda \phi(x, y)
\]
\[
    \begin{cases}
        L_x'(x, y) = 0 \\
        L_y'(x, y) = 0 \\
        \phi(x, y) = 0
    \end{cases}
\]

\subsection{Multiple Integrals}

\[
    \iint_D f(x, y) dx dy = \iint_{D'} f(x(u, v), y(u, v)) \det(\mathbf{J}) du dv
\]

\subsubsection{Double Integral}

\textbf{Cartesian Coordinate System:}
\[
    \iint_D f(x, y) d\sigma = \int_c^d dy \int_{\psi_1(y)}^{\psi_2(y)} f(x, y) dx
\]
\textbf{Polar Coordinate System:}
\[
    \iint_D f(x, y) dx dy = \iint_D f(\rho \cos \theta, \rho \sin \theta) \rho d\rho d\theta = \int_\alpha^\beta d\theta \int_{\phi_1(\theta)}^{\phi_2(\theta)} f(\rho \cos \theta, \rho \sin \theta) \rho d\rho
\]

\subsubsection{Triple Integral}

\textbf{Cartesian Coordinate System}
\[
    \iiint_\Omega f(x, y, z) dv = \int_a^b dx \int_{y_1(x)}^{y_2(x)} dy \int_{z_1(x, y)}^{z_2(x, y)} f(x, y, z) dz
\]
\textbf{Cylindrical Coordinate System}
\[
    \begin{cases}
        x = \rho \cos \theta \\
        y = \rho \sin \theta \\
        z = z
    \end{cases}
\]
\[
    \iiint_\Omega f(x, y, z) dv = \iiint_\Omega F(\rho, \theta, z) \rho d\rho d\theta dz
\]
\textbf{Spherical Coordinate System}
\[
    \begin{cases}
        x = r \sin \phi \cos \theta \\
        y = r \sin \phi \sin \theta \\
        z = r \cos \phi
    \end{cases}
\]
\[
    \iiint_\Omega f(x, y, z) dv = \iiint_\Omega F(r, \phi, \theta) r^2 \sin \phi dr d\phi d\theta
\]

\subsection{Line Integral}

\subsubsection{Line Integrals of a Scalar Field}

For parametric curve:
\[
    \begin{cases}
        x = \phi(t) \\
        y = \psi(t) \\
        z = \omega(t)
    \end{cases}
\]
\[
    \int_\Gamma f(x, y, z) ds = \int_\alpha^\beta f(\phi(t), \psi(t), \omega(t)) \sqrt{\phi'(t)^2 + \psi'(t)^2 + \omega'(t)^2} dt
\]

\subsubsection{Line Integrals of a Vector Field}

\[
    \int_\Gamma P(x, y, z) dx + Q(x, y, z) dy + R(x, y, z) dz =
\]
\[
    \int_\alpha^\beta \left[P(\phi(t), \psi(t), \omega(t)) \phi'(t) + Q(\phi(t), \psi(t), \omega(t)) \psi'(t) + R(\phi(t), \psi(t), \omega(t)) \omega'(t)\right] dt
\]

\subsubsection{Conversion between two types of Line Integrals}

\[
    \boldsymbol{\tau} = \phi'(t) \mathbf{i} + \psi'(t) \mathbf{j} + \omega'(t) \mathbf{k}
\]
\[
    \int_\Gamma P dx + Q dy + R dz = \int_\Gamma (P \cos \alpha + Q \cos \beta + R \cos \gamma) ds
\]

\subsubsection{Green's Theorem}

\[
    \iint_D \left(\frac{\partial Q}{\partial x} - \frac{\partial P}{\partial y}\right) dx dy = \oint_L P dx + Q dy
\]

\subsubsection{Area}

\[
    A = \frac{1}{2} \oint_L x dy - y dx
\]

\subsubsection{Path Independence for Line Integrals of a Vector Field}

\[
    \frac{\partial Q}{\partial x} = \frac{\partial P}{\partial y}
\]

\subsubsection{Exact Differential Equation}

\[
    P(x, y) dx + Q(x, y) dy = 0
\]
\[
    \frac{\partial Q}{\partial x} = \frac{\partial P}{\partial y}
\]
\[
    u(x, y) = \int_{(x_0, y_0)}^{(x, y)} P(x, y) dx + Q(x, y) dy = C
\]

\subsection{Surface Integral}

\subsubsection{Surface Integral of a Scalar Field}

\[
    \iint_\Sigma f(x, y, z) dS = \iint_{D_{xy}} f(x, y, z(x, y)) \sqrt{1 + z_x'(x, y)^2 + z_y'(x, y)^2} dx dy
\]

\subsubsection{Surface Integral of a Vector Field}

\[
    \iint_\Sigma f(x, y, z) dx dy = \pm \iint_{D_{xy}} f(x, y, z(x, y)) dx dy
\]

\subsubsection{Conversion between two types of Surface Integrals}

\[
    \cos \alpha = \frac{-z_x'}{\sqrt{1 + z_x'^2 + z_y'^2}}
\]
\[
    \cos \beta = \frac{-z_y'}{\sqrt{1 + z_x'^2 + z_y'^2}}
\]
\[
    \cos \gamma = \frac{1}{\sqrt{1 + z_x'^2 + z_y'^2}}
\]
\[
    \iint_\Sigma P dy dz + Q dz dx + R dx dy = \iint_\Sigma (P \cos \alpha + Q \cos \beta + R \cos \gamma) dS
\]

\subsubsection{Divergence Theorem}

\[
    \iiint_\Omega \left(\frac{\partial P}{\partial x} + \frac{\partial Q}{\partial y} + \frac{\partial R}{\partial z}\right) dv = \iint_\Sigma P dy dz + Q dz dx + R dx dy
\]

\newpage
\section{Coordinate Transformation}

\subsection{Inner Product}

\[
    \langle f(x), g(x) \rangle = \int_a^b f(x) g(x) dx
\]

\subsection{Norm}

\[
    \|f(x)\| = \sqrt{\langle f(x), f(x) \rangle}
\]
In Complex Field:
\[
    \langle f(x), g(x) \rangle = \int_a^b f(x) \overline{g(x)} dx
\]

\subsection{Eigen Function}

\[
    \frac{d^n}{dx^n} e^{inx} = (in)^n e^{inx}
\]

\subsection{Fourier Analysis}

Express a function as a sum of projections onto a set of orthogonal eigenfunctions.

\subsubsection{Fourier Series}

A function $f(t)$ with period $2\pi$ can be represented as:
\[
    f(t) = \frac{a_0}{2} + \sum_{n=1}^{\infty} \left[a_n \cos(nt) + b_n \sin(nt)\right]
\]
\[
    a_n = \frac{\langle f(t), \cos(nt) \rangle}{\|\cos(nt)\|^2} = \frac{1}{\pi} \int_{-\pi}^{\pi} f(t) \cos(nt) dt
\]
\[
    b_n = \frac{\langle f(t), \sin(nt) \rangle}{\|\sin(nt)\|^2} = \frac{1}{\pi} \int_{-\pi}^{\pi} f(t) \sin(nt) dt
\]
In Complex Field:
\[
    f(t) = \sum_{n=-\infty}^{\infty} c_n e^{int}
\]
\[
    c_n = \frac{\langle f(t), e^{int} \rangle}{\|e^{int}\|^2} = \frac{1}{2\pi} \int_{-\pi}^{\pi} f(t) e^{-int} dt
\]
\[
    a_n = c_n + c_{-n}
\]
\[
    b_n = i(c_n - c_{-n})
\]

\subsubsection{Fourier Transform}

\[
    F(\omega) = \mathcal{F}(f(x)) = \int_{-\infty}^{\infty} f(t) e^{-i\omega t} dt
\]
\[
    f(t) = \mathcal{F}^{-1}(F(\omega)) = \frac{1}{2\pi} \int_{-\infty}^{\infty} F(\omega) e^{i\omega t} dt
\]
\textbf{Properties:}
\[
    \mathcal{F}\left(\frac{d^n}{dt^n} f(t)\right) = (i\omega)^n F(\omega)
\]

\subsection{Laplace Transform}

\[
    F(s) = \mathcal{L}(f(t)) = \int_0^{\infty} f(t) e^{-st} dt
\]
\[
    f(t) = \frac{1}{2\pi i} \int_{\gamma - i\infty}^{\gamma + i\infty} F(s) e^{st} ds
\]
\textbf{Derivation:}
\[
    \mathcal{L}(f(t)) = \mathcal{F}(f(t) e^{-\gamma t} H(t))
\]
where:
\[
    s = \gamma + i\omega
\]
\[
    H(t) = \begin{cases}
        0, & t < 0 \\
        1, & t \geq 0
    \end{cases}
\]

\subsection{Convolution}

\[
    (f * g)(t) = \int_{-\infty}^{\infty} f(\tau) g(t - \tau) d\tau
\]
\[
    \mathcal{F}(f * g) = \mathcal{F}(f) \cdot \mathcal{F}(g)
\]
\[
    \mathcal{L}(f * g) = \mathcal{L}(f) \cdot \mathcal{L}(g)
\]

\end{document}
